theories/ctx.v
@@ -1,0 +1,221 @@
+From mathcomp Require Import all_ssreflect.
+
+Section Lookup.
+  Set Implicit Arguments.
+  Variables (K : eqType) (V : Type).
+
+  Definition remove k (L : seq (K*V)) := filter (fun y => k != y.1) L.
+  
+  (* get the first value (option) for key k *)
+  Fixpoint lookup (k : K) (l : seq (K * V)) : option V :=
+    match l with
+    | [::] => None
+    | (k',v)::xs => if k' == k then Some v else lookup k xs
+    end.
+
+  Definition key_absent k (l: seq (K * V)) := 
+    match lookup k l with None => true | _ => false end.
+
+  Fixpoint valid_sig (L : seq (K*V)) :=
+    match L with
+    | [::] => true
+    | x::xs => key_absent x.1 xs && valid_sig xs
+    end.
+
+  Fixpoint add k v l : (seq (K*V)) :=
+    match l with
+    | [::] => [::(k, v)]
+    | x :: xs => if x.1 == k then (k, v) :: xs else x :: add k v xs
+    end.
+
+  Lemma valid_sig_add_diff {k k' v' l}:
+    size [seq y <- l | k == y.1] = 0 ->
+      k <> k' ->
+        size [seq y <- add k' v' l | k == y.1] = 0.
+  Proof.
+    elim: l k k' v' => //=.
+      move=> k k' v' _; case: eqP => //.
+    move=> [k v] l IH k1 k2 v'.
+    case:eqP => //= H1 H2 H3.
+    have IH' := IH _ _ _ H2 H3.
+    case:eqP => //= H4; subst; case: eqP => //=.
+  Qed.
+
+  Lemma key_absent_add_diff {k k' v} l:
+    k <> k' -> key_absent k' (add k v l) = key_absent k' l.
+  Proof.
+    rewrite/key_absent.
+    elim: l k k' v => //=[|[k v]xs IH] k1 k2 v1//=; repeat case: eqP => //=; try congruence.
+    move=> H1 H2 H3.
+    by apply: IH.
+  Qed.
+
+  Lemma valid_sig_add {l k v}:
+    valid_sig l -> valid_sig (add k v l).
+  Proof.
+    elim: l k v => //= [[k v]] l IH k' v'/= /andP[H1 H2].
+    case:eqP => H3; subst => /=.
+      rewrite H1//.
+    rewrite IH//andbT key_absent_add_diff//; congruence.
+  Qed.
+
+  Goal forall k v l, size (add k v l) <> 0.
+  Proof. move=> ??[]//=*; case: ifP => //. Qed.
+
+End Lookup.
+Arguments lookup {_ _}.
+Arguments remove {_ _}.
+Arguments add {_ _}.
+Arguments valid_sig {_ _}.
+Arguments key_absent {_ _}.
+
+
+
+Section lookup.
+  Lemma key_absent_remove {T: eqType} {K:Type} {k} {l: seq (T*K)}:
+    (key_absent k l) -> remove k l = l.
+  Proof.
+    rewrite/key_absent.
+    elim: l k => //= [[k v]] xs IH k'; case: eqP => //= H1 H2.
+    rewrite IH//.
+    case:eqP => //; congruence.
+  Qed.
+
+  Lemma lookup_remove_None {T: eqType} {K:Type} {k} {l: seq (T*K)}:
+    (lookup k (remove k l)) = None.
+  Proof.
+    elim: l k => //= -[k v] l IH k'/=.
+    case:eqP => //= H; rewrite IH; case: eqP; congruence.
+  Qed.
+
+  Lemma lookup_remove_diff {T: eqType} {K:Type} {k k'} {l: seq (T*K)}:
+     k' <> k ->
+      lookup k (remove k' l) = lookup k l.
+  Proof.
+    elim: l k k' => //= -[k v] l IH k1 k2 H.
+    case:eqP => //= H1; subst.
+      by case:eqP => //= _; apply: IH.
+    case: eqP => //= H2; subst.
+    by apply: IH.
+  Qed.
+
+  Lemma remove_comm {T: eqType} {K:Type} {x y} {l: seq (T*K)}:
+    remove x (remove y l) = remove y (remove x l).
+  Proof.
+    elim: l x y => //= -[k v] xs IH/= x y.
+    case: eqP => H/=; subst.
+      case: eqP => H1/=; subst.
+        apply: IH.
+      rewrite eqxx/=; apply: IH.
+    case:eqP => //=H1; subst.
+    case:eqP => //= _; f_equal.
+    apply: IH.
+  Qed.
+
+  Lemma lookup_cat {T : eqType} {K:Type} {k} {X Y : seq (T * K)}:
+      lookup k (X ++ Y) = 
+        if key_absent k X then lookup k Y
+        else lookup k X.
+  Proof.
+    rewrite/key_absent.
+    elim: X k Y => [|[k v] xs IH] k' ys//=.
+    case:eqP => //<-{k'}.
+  Qed.
+
+  Lemma valid_sig_cat {T : eqType} {K:Type} {k} {X Y : seq (T * K)}:
+      valid_sig (X ++ k ::  Y) ->
+        key_absent k.1 X.
+  Proof.
+    rewrite/key_absent.
+    elim: X k Y => //= [[k v] xs] IH [k' v'] ys/= /andP[H1 H2].
+    have/= {IH}:= IH _ _ H2.
+    move: H1; rewrite/key_absent.
+    rewrite lookup_cat.
+    rewrite/key_absent.
+    case:eqP => H//; subst.
+    case: lookup => //=.
+    by rewrite eqxx.
+  Qed.
+
+  Lemma add2  {T: eqType} {K:Type} {k v v1} {A:seq (T*K)} : add k v (add k v1 A) = add k v A.
+  Proof.
+    elim: A k v v1 => //=[|[k v] xs IH] k' v' v2/=.
+      rewrite eqxx => //.
+    case: eqP => //= H; subst.
+      rewrite eqxx//=.
+    case: eqP => //=; rewrite IH//.
+  Qed.
+
+  Lemma add_cat {T: eqType} {K:Type} (L: seq (T*K)) {k v1 v2 xs}:
+    key_absent k L ->
+    add k v1 (L ++ (k, v2) :: xs) = (L ++ (k, v1) :: xs).
+  Proof.
+    rewrite/key_absent.
+    elim: L k v1 v2 xs => //= [|[k v]xs IH] k1 v1 v2 ys/=.
+      by rewrite eqxx.
+    case: eqP => H//; subst.
+    move=> /IH->//.
+  Qed.
+
+  Lemma lookup_add_same {T: eqType} {K:Type} {S: seq (T*K)} {k v}:
+    lookup k (add k v S) = Some v.
+  Proof.
+    elim: S k v => //= [|[k v] xs IH] k1 k2/=; case: eqP => //= H; subst; case: eqP => //.
+  Qed.
+
+  Lemma lookup_add_Some {T: eqType} {K:Type} {S: seq (T*K)} {k k' v' v}:
+    lookup k (add k' v' S) = Some v ->
+      if k' == k then v = v'
+      else lookup k S = Some v.
+  Proof.
+    elim: S k k' v v' => //=[|[k v] xs IH] k1 k2 v1 v2.
+    - case: eqP => //=; congruence.
+    - case: eqP => /= H; subst.
+        case: eqP => //=; congruence.
+      case: eqP => //= H1; subst.
+        case: eqP => //=; congruence.
+      apply: IH.
+  Qed.
+
+  Lemma lookup_add_diff {T: eqType} {K:Type} {k k' v} {S: seq (T*K)}:
+      k <> k' -> lookup k' (add k v S) = lookup k' S.
+  Proof.
+    elim: S k k' v => //= [|[k v] xs IH] k1 k2 v1/=.
+      case:eqP => //=.
+    case:eqP => H1 => //= H2.
+      repeat case:eqP => //=; congruence.
+    (repeat case: eqP) => // H.
+    by apply: IH.
+  Qed.
+
+  Lemma lookup_add_Some2 {T: eqType} {K:Type} {kB k'} k v {S: seq (T*K)}:
+    lookup k' S = Some kB ->
+    exists kB',
+      lookup k' (add k v S) = Some kB'.
+  Proof.
+    elim: S k k' kB v => [|[k v] xs IH]//= k1 k2 v1 v2/=.
+    case: eqP => H1//=; subst.
+      move=> [?]; subst.
+      case: eqP => H; subst => /=; rewrite eqxx; by eexists.
+    case: eqP => H2 H3; subst => /=; case: eqP => H4; subst => //.
+      by rewrite H3; eexists.
+    by apply: IH H3.
+  Qed.
+
+  Lemma add_comm {T: eqType} {K:Type} {k1 k2 m1 m2}  {S: seq (T*K)}:
+    k1 <> k2 -> add k1 m1 (add k2 m2 S) = add k2 m2 (add k1 m1 S).
+  Proof.
+    elim: S k1 k2 m1 m2 => //=[|[k v]xs IH] k1 k2 m1 m2 H/=.
+      do 2 case: eqP => //=; try congruence.
+      admit. (*should be ok by ordering element*)
+    case eqP => //=H1; subst.
+      repeat case: eqP; try congruence.
+      move=> /=.
+      rewrite eqxx//.
+    repeat case: eqP => /=; try congruence.
+    move=> H3 H4.
+    by f_equal; apply: IH.
+  Admitted.
+  
+End lookup.
+
